doubly linked list (partial)

examples/steel/DList.fst
@@ -4,50 +4,9 @@ open Steel.Effect
 open Steel.FractionalPermission
 open Steel.Reference
 open DList.Invariant
-
-assume val p : slprop u#1
-assume val q : slprop u#1
-assume val r : slprop u#1
-assume val s : slprop u#1
-assume val sladmit (#[@@framing_implicit] p:slprop)  (#[@@framing_implicit]q:slprop) (_:unit) : SteelT unit p (fun _ -> q)
-
-let test_pq () : SteelT unit p (fun _ -> q) = sladmit()
-let test_pr () : SteelT unit p (fun _ -> r) = test_pq(); sladmit()
-let test_rs () : SteelT unit r (fun _ -> s) = sladmit()
-let test_ps () : SteelT unit p (fun _ -> s) = test_pq(); sladmit(); test_rs()
-
-let test_pr2 () : SteelT unit p (fun _ -> r) = let x = test_pq() in sladmit()
-
-assume val sladmitf (#[@@framing_implicit] p:slprop)  (#[@@framing_implicit]q:slprop) (_:unit) : SteelF unit p (fun _ -> q) (fun _ -> True) (fun _ _ _ -> True)
+open Utils
 
 
-let test_pq_f () : SteelT unit p (fun _ -> q) = sladmitf()
-let test_pr_f () : SteelT unit p (fun _ -> r) = test_pq(); sladmitf()
-let test_rs_f () : SteelT unit r (fun _ -> s) = sladmit()
-let test_ps_f () : SteelT unit p (fun _ -> s) = test_pq(); sladmitf(); test_rs()
-
-let test_pr2_f () : SteelT unit p (fun _ -> r) = let x = test_pq() in sladmitf()
-
-assume val sladmit_dep (#a:_)
-                       (p:slprop)              
-                       (q:(a -> slprop))
-       : SteelT a p q
-
-assume val sladmit_depF (#a:_)
-                       (#[@@framing_implicit] p:slprop)              
-                       (#[@@framing_implicit] q:(a -> slprop))
-                       (_:unit)
-       : SteelF a p q (fun _ -> True) (fun _ _ _ -> True)
-
-let return (#a:_)
-                    (p:slprop)              
-                    (q:(a -> slprop))
-                    (x:a) 
-    : Steel a p q
-         (requires fun _ -> p == q x)
-         (ensures fun _ y _ -> y == x)
-    = change_slprop p (q x) (fun _ -> ());
-      x
 //We're trying to write this library in the "internal" language of Steel
 //the front end + frame inference should elaborate into something like this
 //If it does, then the proofs can be done with almost nothing in the SMT context
@@ -69,9 +28,7 @@ let new_dlist (#a:Type) (init:a)
                   (fun _ -> ());
     intro_dlist_cons null_dlist p null_dlist cell [];
     let pc = p, cell in
-    return (dlist null_dlist p null_dlist [cell])
-           (fun pc -> dlist null_dlist (fst pc) null_dlist [(snd pc)])
-           pc
+    return pc
 
 let read_head (#a:_) (from0:t a) (ptr0:t a) (to0: t a)
               (hd:cell a)
@@ -98,34 +55,45 @@ let read_head (#a:_) (from0:t a) (ptr0:t a) (to0: t a)
 
      c0
 
-let rec datas (l:list (cell 'a)) : list 'a =
-  match l with
-  | [] -> []
-  | hd::tl -> data hd::datas tl
+let set_prev (c:cell 'a) (prev: t 'a)
+  : Tot (cell 'a)
+  = mk_cell prev (next c) (data c)
 
-assume
-val datas_append (l0 l1:list (cell 'a))
-  : Lemma (datas (l0 @ l1) == datas l0 @ datas l1)
-          [SMTPat (datas (l0 @ l1))]
+let set_next (c:cell 'a) (next: t 'a)
+  : Tot (cell 'a)
+  = mk_cell (prev c) next (data c)
 
-assume
-val append_cons (#a:_) (hd : cell a) (l0 l1:list (cell a))
-  : Lemma (data hd :: datas (l0 @ l1) == datas (hd::l0) @ datas l1)
-          [SMTPat (data hd :: datas (l0 @ l1))]
+let intro_dlist_cons (#a:Type) (left:t a)
+                               (ptr:t a)
+                               (right:t a)
+                               (hd: cell a)
+                               (ptr1 : t a)
+                               (tl: list (cell a))
+   : Steel unit
+     (pts_to ptr full_perm hd `star` dlist ptr ptr1 right tl)
+     (fun _ -> dlist left ptr right (hd::tl))
+     (requires fun _ ->
+       prev hd == left /\
+       next hd == ptr1 /\
+       ptr =!= right)
+     (ensures fun _ _ _ -> True)
+   = change_slprop (dlist ptr ptr1 right tl)
+                   (dlist ptr (next hd) right tl)
+                   (fun _ -> ());
+     intro_dlist_cons left ptr right hd tl
 
-// let test (r:resource) (c:cell unit) : St (t unit) r (fun p -> r <*> pts_to p c) =
-//   frame r
-//         (fun p -> r <*> pts_to p c)
-//         (fun _ -> alloc_cell c)
+let write_prev (#a:_) (#from0:t a) (ptr0:t a) (#to0: t a)
+               (#hd:cell a)
+               (#tl:list (cell a))
+               (prev:t a)
+    : SteelT unit
+      (dlist from0 ptr0 to0 (hd::tl))
+      (fun _ -> dlist prev ptr0 to0  (set_prev hd prev :: tl))
+    = elim_dlist_cons _ ptr0 _ _ _;
+      write ptr0 (set_prev hd prev);
+      intro_dlist_cons _ ptr0 _ _ _ _
 
-// let drop (r:resource)
-//   : St unit
-//     (requires r)
-//     (ensures fun _ -> empty_resource)
-//   = reveal_empty_resource()
-
-assume
-val concat_nil_l (#a:Type)
+let concat_nil_l (#a:Type)
                  (from0:t a) (ptr0:t a) (to0: t a) (hd:cell a) (tl0:list (cell a))
                  (from1:t a) (ptr1:t a) (hd1:cell a) (tl1:list (cell a))
    : Steel (list (cell a))
@@ -137,17 +105,35 @@ val concat_nil_l (#a:Type)
        prev hd == from0 /\
        to0 =!= ptr0)
      (ensures fun _ _ _ -> True)
+   = assume (ptr0 =!= null_dlist);
+   
+     // 1. invert dlist tl0 to dlist []
+     invert_dlist_nil_eq ptr0 to0 to0 tl0;
+     drop (dlist ptr0 to0 to0 []);
+     // tl0 == []
+     
+     // 2. ptr0.next <- ptr1
+     write ptr0 (set_next hd ptr1);
 
+     write_prev ptr1 ptr0;
+
+     intro_dlist_cons from0 ptr0 _ _ ptr1 _;
+
+     drop (pure (tl0 == []));
+     return (set_next hd ptr1
+             :: set_prev hd1 ptr0 
+             :: tl1)
+     
 let concat_t a =
-  (from0:t a) ->
+  (#[@@framing_implicit] from0:t a) ->
+  (#[@@framing_implicit] to0: t a) ->
+  (#[@@framing_implicit] hd0:cell a) ->
+  (#[@@framing_implicit] tl0:list (cell a)) ->
+  (#[@@framing_implicit] from1:t a) ->
+  (#[@@framing_implicit] hd1:cell a) ->
+  (#[@@framing_implicit] tl1:list (cell a)) ->
   (ptr0:t a) ->
-  (to0: t a) ->
-  (hd0:cell a) ->
-  (tl0:list (cell a)) ->
-  (from1:t a) ->
   (ptr1:t a) ->
-  (hd1:cell a) ->
-  (tl1:list (cell a)) ->
   SteelT (list (cell a))
      (dlist from0 ptr0 to0 (hd0::tl0) `star`
       dlist from1 ptr1 null_dlist (hd1::tl1))
@@ -171,20 +157,26 @@ let concat_cons (#a:Type) (aux:concat_t a)
      change_slprop (dlist ptr0 (next c0) to0 tl0)
                    (dlist ptr0 (next c0) to0 (hd0::tl0'))
                    (fun _ -> ());
-     let l = aux ptr0 (next c0) to0 hd0 tl0' from1 ptr1 hd1 tl1 in
+     let l = aux (next c0) ptr1 in
      assume (ptr0 =!= null_dlist);
-     intro_dlist_cons from0 ptr0 null_dlist c0 l;
+     intro_dlist_cons from0 ptr0 _ _ (next c0) _;
      c0::l
 
 let rec concat (#a:Type)
-               (from0:t a) (ptr0:t a) (to0: t a) (hd0:cell a) (tl0:list (cell a))
-               (from1:t a) (ptr1:t a) (hd1:cell a) (tl1:list (cell a))
+               (#[@@framing_implicit] from0:t a) 
+               (#[@@framing_implicit] to0: t a)
+               (#[@@framing_implicit] hd0:cell a)
+               (#[@@framing_implicit] tl0:list (cell a))
+               (#[@@framing_implicit] from1:t a) 
+               (#[@@framing_implicit] hd1:cell a)
+               (#[@@framing_implicit] tl1:list (cell a))
+               (ptr0:t a)
+               (ptr1:t a) 
    : SteelT (list (cell a))
      (dlist from0 ptr0 to0 (hd0::tl0) `star`
       dlist from1 ptr1 null_dlist (hd1::tl1))
      (fun l ->
        dlist from0 ptr0 null_dlist l)
-//       datas l == datas l0 @ datas l1)
    =
      let to1 = null_dlist #a in
 
@@ -222,135 +214,38 @@ let rec concat (#a:Type)
          concat_cons (concat #a) 
                      from0 ptr0 to0 c0 tl0
                      from1 ptr1 hd1 tl1)
-         // invert_dlist_cons_neq ptr0 (next c0) to0 tl0;
-         // let l = concat ptr0 (next c0) to0 tl0 from1 ptr1 hd1 l1 in
-         // sladmit_depF #_ 
-         //              #(pts_to ptr0 full_perm c0 `star`
-         //                dlist ptr0 (next c0) null_dlist l)
-         //              #(dlist from0 ptr0 null_dlist) 
-         //              ())
 
-//      if ptr_eq (next c0) to0
-//      then begin //we are at the end of l0
-//        // 3. invert dlist tl0 to dlist []
-//        frame
-//          (pts_to ptr0 hd0 <*> dlist ptr0 (next hd0) to0 tl0 <*> dlist from1 ptr1 to1 l1)
-//          (fun _ -> pts_to ptr0 hd0 <*> dlist ptr0 to0 to0 [] <*> dlist from1 ptr1 to1 l1)
-//          (fun _ -> invert_dlist_nil_eq ptr0 (next hd0) to0 tl0);
+let snoc (#a:Type)
+         (#[@@framing_implicit] from0:t a)
+         (#[@@framing_implicit] to0: t a)
+         (#[@@framing_implicit] hd0:cell a)
+         (#[@@framing_implicit] l0:list (cell a))
+         (ptr0:t a)
+         (v:a)
+   : SteelT (list (cell a))
+     (requires
+       dlist from0 ptr0 to0 (hd0::l0))
+     (ensures
+       dlist from0 ptr0 null_dlist)
+     // (requires fun _ ->
+     //   Cons? l0)
+     // (ensures fun _ l _ ->
+     //   datas l == datas l0 @ datas [mk_cell null_dlist null_dlist v])
+   = let tl = new_dlist v in
+     concat #_ #_ #_ #_ #_ #null_dlist #(snd tl) #[] ptr0 (fst tl)
 
-//        frame
-//          (pts_to ptr0 hd0 <*> dlist ptr0 to0 to0 [] <*> dlist from1 ptr1 to1 l1)
-//          (fun _ -> pts_to ptr0 hd0 <*> dlist from1 ptr1 to1 l1)
-//          (fun _ -> drop (dlist ptr0 to0 to0 []));
-
-//        // This is a long-winded way of saying:
-//        //   p0.next <- p1
-//        let c0' = mk_cell (prev c0) ptr1 (data c0) in
-//        frame
-//            (pts_to ptr0 hd0 <*> dlist from1 ptr1 to1 l1)
-//            (fun _ -> pts_to ptr0 c0' <*> dlist from1 ptr1 to1 l1)
-//            (fun _ -> write_ptr ptr0 hd0 c0');
-
-
-//        let c1 =
-//          frame
-//            (pts_to ptr0 c0' <*> dlist from1 ptr1 to1 (hd1::tl1))
-//            (fun _ -> pts_to ptr0 c0' <*> dlist from1 ptr1 to1 (hd1::tl1))
-//            (fun _ -> read_head from1 ptr1 to1 hd1 tl1) in
-
-
-//        frame
-//            (pts_to ptr0 c0' <*> dlist from1 ptr1 to1 (hd1::tl1))
-//            (fun _ -> pts_to ptr0 c0' <*> pts_to ptr1 hd1 <*> dlist ptr1 (next hd1) to1 tl1)
-//            (fun _ -> elim_dlist_cons from1 ptr1 to1 hd1 tl1);
-
-//        // This is a long-winded way of saying:
-//        //   p1.prev <- p0
-//        let c1' = mk_cell ptr0 (next c1) (data c1) in
-//        frame
-//            (pts_to ptr0 c0' <*> pts_to ptr1 hd1 <*> dlist ptr1 (next hd1) to1 tl1)
-//            (fun _ -> pts_to ptr0 c0' <*> pts_to ptr1 c1' <*> dlist ptr1 (next hd1) to1 tl1)
-//            (fun _ -> write_ptr ptr1 hd1 c1');
-
-//        frame
-//            (pts_to ptr0 c0' <*> pts_to ptr1 c1' <*> dlist ptr1 (next c1') to1 tl1)
-//            (fun _ -> pts_to ptr0 c0' <*> dlist ptr0 ptr1 to1 (c1'::tl1))
-//            (fun _ -> intro_dlist_cons ptr0 ptr1 to1 c1' tl1);
-
-//        intro_dlist_cons from0 ptr0 to1 c0' (c1'::tl1);
-
-//        let l = [c0'] @ (c1'::tl1) in
-//        assert (datas l1 == data c1' :: datas tl1);
-//        assert (datas l == datas [c0'] @ datas (c1'::tl1));
-//        assert (datas (l0 @ l1) == datas l0 @ datas l1);
-//        assert (datas l1 == datas (c1' :: tl1));
-//        assert (datas l0 == datas [c0']);
-//        assert (datas l == datas l0 @ datas l1);
-//        l
-//      end
-//      else begin
-//        //pts_to ptr0 hd0 <*> dlist ptr0 (next hd0) to0 tl0 <*> dlist from1 ptr1 to1 l1
-//        //next c0 =!= t0
-//        frame
-//           (pts_to ptr0 hd0 <*> dlist ptr0 (next c0) to0 tl0 <*> dlist from1 ptr1 null_dlist l1)
-//           (fun _ -> pts_to ptr0 hd0 <*> dlist ptr0 (next c0) to0 tl0 <*> dlist from1 ptr1 null_dlist l1)
-//           (fun _ -> invert_dlist_cons_neq ptr0 (next c0) to0 tl0);
-
-//        let l =
-//          frame
-//            (pts_to ptr0 hd0 <*> dlist ptr0 (next c0) to0 tl0 <*> dlist from1 ptr1 null_dlist l1)
-//            (fun l -> pts_to ptr0 hd0 <*> dlist ptr0 (next c0) null_dlist l)
-//            (fun _ -> concat ptr0 (next c0) to0 tl0 from1 ptr1 l1)
-//        in
-//        intro_dlist_cons from0 ptr0 null_dlist hd0 l;
-//        resource_assertion (dlist from0 ptr0 to1 (hd0::l));
-//        assert (datas l == datas tl0 @ datas l1);
-//        assert (datas (hd0::l) == data hd0 :: datas (tl0 @ l1));
-//        append_cons hd0 tl0 l1;
-//        hd0::l
-//      end
-
-// let snoc (#a:Type)
-//          (from0:t a) (ptr0:t a) (to0: t a) (l0:list (cell a))
-//          (v:a)
-//    : Steel (list (cell a))
-//      (requires
-//        dlist from0 ptr0 to0 l0)
-//      (ensures
-//        dlist from0 ptr0 null_dlist)
-//      (requires fun _ ->
-//        Cons? l0)
-//      (ensures fun _ l _ ->
-//        datas l == datas l0 @ datas [mk_cell null_dlist null_dlist v])
-//    = let pc =
-//        frame (dlist from0 ptr0 to0 l0)
-//              (fun pc -> dlist from0 ptr0 to0 l0 <*> dlist null_dlist (fst pc) null_dlist [snd pc])
-//              (fun _ -> new_dlist v) in
-
-//      concat from0 ptr0 to0 l0
-//             null_dlist (fst pc) [snd pc]
-
-// let cons (#a:Type)
-//          (from0:t a) (ptr0:t a) (l0:list (cell a))
-//          (v:a)
-//    : Steel (t a & list (cell a))
-//      (requires
-//        dlist from0 ptr0 null_dlist l0)
-//      (ensures fun pc ->
-//        dlist null_dlist (fst pc) null_dlist (snd pc))
-//      (requires fun _ ->
-//        Cons? l0)
-//      (ensures fun _ pc _ ->
-//        datas (snd pc) == datas [mk_cell null_dlist null_dlist v] @ datas l0)
-//    = let to0 = null_dlist in
-
-//      let pc =
-//        frame (dlist from0 ptr0 to0 l0)
-//              (fun pc -> dlist null_dlist (fst pc) null_dlist [snd pc] <*> dlist from0 ptr0 to0 l0)
-//              (fun _ -> new_dlist v) in
-
-//      let l =
-//        concat null_dlist (fst pc) null_dlist [snd pc]
-//               from0 ptr0 l0
-//      in
-//      fst pc, l
+let cons (#a:Type)
+         (from0:t a) (ptr0:t a) (hd0:cell a) (l0:list (cell a))
+         (v:a)
+   : SteelT (t a & list (cell a))
+     (requires
+       dlist from0 ptr0 null_dlist (hd0::l0))
+     (ensures fun pc ->
+       dlist null_dlist (fst pc) null_dlist (snd pc))
+     // (requires fun _ ->
+     //   Cons? l0)
+     // (ensures fun _ pc _ ->
+     //   datas (snd pc) == datas [mk_cell null_dlist null_dlist v] @ datas l0)
+   = let pc = new_dlist v in
+     let l = concat #_ #null_dlist #null_dlist #(snd pc) #[] (fst pc) ptr0 in
+     fst pc, l
